@prefix exif:    <http://www.kanzaki.com/ns/exif#> .
@prefix nid3:    <http://www.semanticdesktop.org/ontologies/2007/05/10/nid3#> .
@prefix nrl:     <http://www.semanticdesktop.org/ontologies/2007/08/15/nrl#> .
@prefix nfo:     <http://www.semanticdesktop.org/ontologies/2007/03/22/nfo#> .
@prefix xsd:     <http://www.w3.org/2001/XMLSchema#> .
@prefix tmo:     <http://www.semanticdesktop.org/ontologies/2008/05/20/tmo#> .
@prefix protege:  <http://protege.stanford.edu/system#> .
@prefix nmo:     <http://www.semanticdesktop.org/ontologies/2007/03/22/nmo#> .
@prefix rdfs:    <http://www.w3.org/2000/01/rdf-schema#> .
@prefix nexif:   <http://www.semanticdesktop.org/ontologies/2007/05/10/nexif#> .
@prefix ncal:    <http://www.semanticdesktop.org/ontologies/2007/04/02/ncal#> .
@prefix pimo:    <http://www.semanticdesktop.org/ontologies/2007/11/01/pimo#> .
@prefix dcterms:  <http://purl.org/dc/terms/> .
@prefix nao:     <http://www.semanticdesktop.org/ontologies/2007/08/15/nao#> .
@prefix geo:     <http://www.w3.org/2003/01/geo/wgs84_pos#> .
@prefix dc:      <http://purl.org/dc/elements/1.1/> .
@prefix nie:     <http://www.semanticdesktop.org/ontologies/2007/01/19/nie#> .
@prefix nco:     <http://www.semanticdesktop.org/ontologies/2007/03/22/nco#> .
@prefix rdf:     <http://www.w3.org/1999/02/22-rdf-syntax-ns#> .

nmo: {nmo:IMMessage
          a       rdfs:Class ;
          rdfs:comment "A message sent with Instant Messaging software." ;
          rdfs:label "IMMessage" ;
          rdfs:subClassOf nmo:MimeEntity , nmo:Message .

    nmo:Email
          a       rdfs:Class ;
          rdfs:comment "An email." ;
          rdfs:label "Email" ;
          rdfs:subClassOf nmo:Message .

    nmo:messageSubject
          a       rdf:Property ;
          rdfs:comment "The subject of a message" ;
          rdfs:domain nmo:Message ;
          rdfs:label "messageSubject" ;
          rdfs:range xsd:string ;
          rdfs:subPropertyOf nie:subject .

    nmo:MessageHeader
          a       rdfs:Class ;
          rdfs:comment "An arbitrary message header." ;
          rdfs:label "MessageHeader" ;
          rdfs:subClassOf rdfs:Resource .

    nmo:references
          a       rdf:Property ;
          rdfs:comment "Signifies that a message references another message. This property is a generic one. See RFC 2822 Sec. 3.6.4" ;
          rdfs:domain nmo:Message ;
          rdfs:label "references" ;
          rdfs:range nmo:Message .

    nmo:to
          a       rdf:Property ;
          rdfs:comment "The primary intended recipient of an email." ;
          rdfs:domain nmo:Email ;
          rdfs:label "to" ;
          rdfs:range nco:Contact ;
          rdfs:subPropertyOf nmo:primaryRecipient .

    nmo:cc
          a       rdf:Property ;
          rdfs:comment "A Contact that is to receive a cc of the email. A cc (carbon copy) is a copy of an email message whose recipient appears on the recipient list, so that all other recipients are aware of it." ;
          rdfs:domain nmo:Email ;
          rdfs:label "cc" ;
          rdfs:range nco:Contact ;
          rdfs:subPropertyOf nmo:secondaryRecipient .

    nmo:from
          a       rdf:Property ;
          rdfs:comment "The sender of the message" ;
          rdfs:domain nmo:Message ;
          rdfs:label "from" ;
          rdfs:range nco:Contact .

    nmo:isRead
          a       rdf:Property ;
          rdfs:comment "A flag that states the fact that a MailboxDataObject has been read." ;
          rdfs:domain nmo:MailboxDataObject ;
          rdfs:label "isRead" ;
          rdfs:range xsd:boolean .

    nmo:Mailbox
          a       rdfs:Class ;
          rdfs:comment "A mailbox - container for MailboxDataObjects." ;
          rdfs:label "Mailbox" ;
          rdfs:subClassOf nie:InformationElement .

    nmo:MailboxDataObject
          a       rdfs:Class ;
          rdfs:comment "An entity encountered in a mailbox. Most common interpretations for such an entity include Message or Folder" ;
          rdfs:label "MailboxDataObject" ;
          rdfs:subClassOf nie:DataObject .

    nmo:messageHeader
          a       rdf:Property ;
          rdfs:comment "Links the message wiith an arbitrary message header." ;
          rdfs:domain nmo:Message ;
          rdfs:label "messageHeader" ;
          rdfs:range nmo:MessageHeader ;
          nrl:maxCardinality "1" .

    nmo:primaryRecipient
          a       rdf:Property ;
          rdfs:comment "The primary intended recipient of a message." ;
          rdfs:domain nmo:Message ;
          rdfs:label "primaryRecipient" ;
          rdfs:range nco:Contact ;
          rdfs:subPropertyOf nmo:recipient .

    nmo:inReplyTo
          a       rdf:Property ;
          rdfs:comment "Signifies that a message is a reply to another message. This feature is commonly used to link messages into conversations. Note that it is more specific than nmo:references. See RFC 2822 sec. 3.6.4" ;
          rdfs:domain nmo:Message ;
          rdfs:label "inReplyTo" ;
          rdfs:range nmo:Message ;
          rdfs:subPropertyOf nmo:references .

    nmo:messageId
          a       rdf:Property ;
          rdfs:comment "An identifier of a message. This property has been inspired by the message-id property defined in RFC 2822, Sec. 3.6.4. It should be used for all kinds of identifiers used by various messaging applications to connect multiple messages into conversations. For email messageids, values are according to RFC2822/sec 3.6.4 and the literal value in RDF must include the brackets." ;
          rdfs:domain nmo:Message ;
          rdfs:label "messageId" ;
          rdfs:range xsd:string ;
          rdfs:subPropertyOf nie:identifier .

    nmo:receivedDate
          a       rdf:Property ;
          rdfs:comment "Date when this message was received." ;
          rdfs:domain nmo:Message ;
          rdfs:label "receivedDate" ;
          rdfs:range xsd:dateTime ;
          rdfs:subPropertyOf dc:date .

    nmo:MimeEntity
          a       rdfs:Class ;
          rdfs:comment "A MIME entity, as defined in RFC2045, Section 2.4." ;
          rdfs:label "MimeEntity" ;
          rdfs:subClassOf nie:InformationElement .

    nmo:replyTo
          a       rdf:Property ;
          rdfs:comment "An address where the reply should be sent." ;
          rdfs:domain nmo:Message ;
          rdfs:label "replyTo" ;
          rdfs:range nco:Contact .

    nmo:recipient
          a       rdf:Property ;
          rdfs:comment "A common superproperty for all properties that link a message with its recipients. Please don't use this property directly." ;
          rdfs:domain nmo:Message ;
          rdfs:label "recipient" ;
          rdfs:range nco:Contact .

    nmo:bcc
          a       rdf:Property ;
          rdfs:comment "A Contact that is to receive a bcc of the email. A Bcc (blind carbon copy) is a copy of an email message sent to a recipient whose email address does not appear in the message." ;
          rdfs:domain nmo:Email ;
          rdfs:label "bcc" ;
          rdfs:range nco:Contact ;
          rdfs:subPropertyOf nmo:secondaryRecipient .

    nmo:secondaryRecipient
          a       rdf:Property ;
          rdfs:comment "A superproperty for all \"additional\" recipients of a message." ;
          rdfs:domain nmo:Message ;
          rdfs:label "secondaryRecipient" ;
          rdfs:range nco:Contact ;
          rdfs:subPropertyOf nmo:recipient .

    nmo:contentMimeType
          a       rdf:Property ;
          rdfs:comment """Key used to store the MIME type of the content of an object when it is different from the object's main MIME type. This value can be used, for example, to model an e-mail message whose mime type is\"message/rfc822\", but whose content has type \"text/html\". If not specified, the MIME type of the
content defaults to the value specified by the 'mimeType' property.""" ;
          rdfs:domain nmo:Email ;
          rdfs:label "contentMimeType" ;
          rdfs:range xsd:string ;
          rdfs:subPropertyOf nie:mimeType .

    nmo:plainTextMessageContent
          a       rdf:Property ;
          rdfs:comment "Plain text representation of the body of the message. For multipart messages, all parts are concatenated into the value of this property. Attachments, whose mimeTypes are different from text/plain or message/rfc822 are considered separate DataObjects and are therefore not included in the value of this property." ;
          rdfs:domain nmo:Message ;
          rdfs:label "plainTextMessageContent" ;
          rdfs:range xsd:string ;
          rdfs:subPropertyOf nie:plainTextContent .

    nmo:Message
          a       rdfs:Class ;
          rdfs:comment "A message. Could be an email, instant messanging message, SMS message etc." ;
          rdfs:label "Message" ;
          rdfs:subClassOf nie:InformationElement .

    nmo:htmlMessageContent
          a       rdf:Property ;
          rdfs:comment "HTML representation of the body of the message. For multipart messages, all parts are concatenated into the value of this property. Attachments, whose mimeTypes are different from text/plain or message/rfc822 are considered separate DataObjects and are therefore not included in the value of this property." ;
          rdfs:domain nmo:Message ;
          rdfs:label "htmlMessageContent" ;
          rdfs:range xsd:string .

    nmo:sentDate
          a       rdf:Property ;
          rdfs:comment "Date when this message was sent." ;
          rdfs:domain nmo:Message ;
          rdfs:label "sentDate" ;
          rdfs:range xsd:dateTime ;
          rdfs:subPropertyOf dc:date , nie:contentCreated ;
          nrl:maxCardinality "1" .

    nmo:sender
          a       rdf:Property ;
          rdfs:comment "The person or agent submitting the message to the network, if other from the one given with the nmo:from property. Defined in RFC 822 sec. 4.4.2" ;
          rdfs:domain nmo:Message ;
          rdfs:label "sender" ;
          rdfs:range nco:Contact ;
          rdfs:subPropertyOf nmo:recipient .

    nmo:headerName
          a       rdf:Property ;
          rdfs:comment "Name of the message header." ;
          rdfs:domain nmo:MessageHeader ;
          rdfs:label "headerName" ;
          rdfs:range xsd:string ;
          nrl:maxCardinality "1" .

    nmo:headerValue
          a       rdf:Property ;
          rdfs:comment "Value of the message header." ;
          rdfs:domain nmo:MessageHeader ;
          rdfs:label "headerValue" ;
          rdfs:range xsd:string ;
          nrl:maxCardinality "1" .

    nmo:hasAttachment
          a       rdf:Property ;
          rdfs:comment "Links a message with files that were sent as attachments." ;
          rdfs:domain nmo:Message ;
          rdfs:label "hasAttachment" ;
          rdfs:range nfo:Attachment ;
          rdfs:subPropertyOf nie:hasPart .
}

<http://www.semanticdesktop.org/ontologies/2007/03/22/nmo_metadata#> {<http://www.semanticdesktop.org/ontologies/2007/03/22/nmo_metadata#>
          a       nrl:GraphMetadata ;
          nrl:coreGraphMetadataFor
                  nmo: .

    nmo:  a       nrl:Ontology ;
          nao:creator <http://www.dfki.uni-kl.de/~mylka> ;
          nao:hasDefaultNamespace
                  "http://www.semanticdesktop.org/ontologies/2007/03/22/nmo#" ;
          nao:hasDefaultNamespaceAbbreviation
                  "nmo" ;
          nao:lastModified "2008-10-05T19:45:56.656Z" ;
          nao:status "Unstable" ;
          nao:updatable "0 " ;
          nao:version "Revision-8" .
}

